
#### The power Rule

$$ \frac{d}{dx} (x^r) = r x^{r-1} $$


#### Exponential Function

$$ \frac{d}{dx} (e^x) = e^x $$

#### General Exponential Function

$$ \frac{d}{dx} (a^x) = (\ln a) a^x $$

#### Natural Logarithm

$$ \frac{d}{dx} (\ln x) = \frac{1}{x} $$

#### Logarithm Base a

$$ \frac{d}{dx} (\log_a x) = \frac{1}{(\ln a)x} $$

#### Sine Function

$$ \frac{d}{dx} (\sin x) = \cos x $$

#### Cosine Function

$$ \frac{d}{dx} (\cos x) = -\sin x $$

#### Tangent Function

$$ \frac{d}{dx} (\tan x) = 1 + \tan^2{x} = \sec^2{x} $$

#### Inverse Sine Function

$$ \frac{d}{dx} (\sin^{-1} x) = \frac{1}{\sqrt{1 - x^2}} $$

#### Inverse Cosine Function

$$ \frac{d}{dx} (\cos^{-1} x) = \frac{-1}{\sqrt{1 - x^2}} $$

#### Inverse Tangent Function

$$ \frac{d}{dx} (\tan^{-1} x) = \frac{1}{1 + x^2} $$

#### Hyperbolic Sine Function

$$ \frac{d}{dx} (\sinh x) = \cosh x $$

#### Hyperbolic Cosine Function

$$ \frac{d}{dx} (\cosh x) = \sinh x $$

#### Hyperbolic Tangent Function

$$ \frac{d}{dx} (\tanh x) = \frac{1}{\cosh^2 x} $$

#### Constant Multiple Rule

$$ (cf(x))' = c f'(x) $$

#### Sum Rule

$$ (f(x) + g(x))' = f'(x) + g'(x) $$

#### Product Rule

$$ (f(x)g(x))' = f(x)g'(x) + g(x)f'(x) $$

#### Quotient Rule

$$ \left( \frac{f(x)}{g(x)} \right)' = \frac{f'(x)g(x) - f(x)g'(x)}{[g(x)]^2} $$